theories/Testing_Pre_orders/Must/Alternative_Preorder/coAcceptance_Set/SoundnessASco.v
@@ -1,0 +1,1227 @@
+(*
+   Copyright (c) 2026 Gaëtan Lopez <glopez@irif.fr>
+
+   Permission is hereby granted, free of charge, to any person obtaining a copy
+   of this software and associated documentation files (the "Software"), to deal
+   in the Software without restriction, including without limitation the rights
+   to use, copy, modify, merge, publish, distribute, sublicense, and/or sell
+   copies of the Software, and to permit persons to whom the Software is
+   furnished to do so, subject to the following conditions:
+
+   The above copyright notice and this permission notice shall be included in all
+   copies or substantial portions of the Software.
+
+   THE SOFTWARE IS PROVIDED "AS IS", WITHOUT WARRANTY OF ANY KIND, EXPRESS OR
+   IMPLIED, INCLUDING BUT NOT LIMITED TO THE WARRANTIES OF MERCHANTABILITY,
+   FITNESS FOR A PARTICULAR PURPOSE AND NONINFRINGEMENT. IN NO EVENT SHALL THE
+   AUTHORS OR COPYRIGHT HOLDERS BE LIABLE FOR ANY CLAIM, DAMAGES OR OTHER
+   LIABILITY, WHETHER IN AN ACTION OF CONTRACT, TORT OR OTHERWISE, ARISING FROM,
+   OUT OF OR IN CONNECTION WITH THE SOFTWARE OR THE USE OR OTHER DEALINGS IN THE
+   SOFTWARE.
+*)
+
+From Stdlib Require ssreflect Setoid.
+From Stdlib.Unicode Require Import Utf8.
+From Stdlib.Lists Require Import List.
+Import ListNotations.
+From Stdlib.Program Require Import Wf Equality.
+From Stdlib.Wellfounded Require Import Inverse_Image.
+
+From stdpp Require Import base countable finite gmap list finite base decidable finite gmap.
+
+From TestingTheory Require Import gLts Bisimulation Lts_OBA Lts_Finite_Output_Chain Lts_FW Lts_OBA_FB Lts_CN
+      Must Subset_Act InteractionBetweenLts ParallelLTSConstruction ForwarderConstruction
+      Termination Convergence WeakTransitions Lift Testing_Predicate DefinitionAS MultisetLTSConstruction.
+From TestingTheory Require Import ActTau InFiniteSetHelper InListPropHelper.
+From TestingTheory Require Import coWeakTransition coConvergence
+      FiniteImageLTS coFiniteImage coSetLTSConstruction DefinitionASco.
+
+(** * Soundness for the co-acceptance-set preorder *)
+
+
+Inductive mustx `{EA : !ExtAction A} `{gLtsT : !gLtsEq T EA} `{TP : @Testing_Predicate T A EA outcome _}
+  `{gLtsP : @gLts P A EA, !Countable P} {Hinter : @Prop_of_Inter P T A dual EA gLtsP _}
+  (X : gset P) (t : T) : Prop :=
+| mx_now (hh : outcome t) : mustx X t
+| mx_step
+    (nh : ¬ outcome t)
+    (ex : forall (p : P), p ∈ X -> ∃ p', inter_step (p, t) τ p')
+    (pt : forall X',
+        lts_tau_set_from_pset_spec1 X X' -> X' ≠ ∅ ->
+        mustx X' t)
+    (et : forall (t' : T), t ⟶ t' -> mustx X t')
+    (com : forall (t' : T) μ (X' : gset P),
+        t ⟶[μ] t' ->
+        cowt_set_from_pset_spec1 X μ X'->
+        X' ≠ ∅ ->
+        mustx X' t')
+  : mustx X t.
+
+#[global] Hint Constructors mustx:mdb.
+Global Notation "X 'must_pass_x' t" := (mustx X t) (at level 70).
+
+Section Must_for_sets.
+
+Context `{EA : !ExtAction A}.
+Context `{gLtsT : !gLtsEq T EA}.
+Context `{TP : @Testing_Predicate T A EA outcome _}.
+Context `{gLtsP : @gLts P A EA, !coFiniteImagegLts P A}.
+Context `{Hinter : @Prop_of_Inter P T A dual EA gLtsP _}.
+
+(** ** Must predicate for Sets *)
+
+Lemma mx_sub X t :
+  X must_pass_x t
+    -> forall X', X' ⊆ X
+      -> X' must_pass_x t.
+Proof.
+  intros hmx. dependent induction hmx.
+  - eauto with mdb.
+  - intros qs sub.
+    apply mx_step; eauto with mdb.
+    + intros qs' hs hneq_nil.
+      set (X' := cowt_tau_set_from_pset_ispec X).
+      destruct X'.
+      eapply H; eauto with mdb.
+      ++ destruct (set_choose_or_empty qs') as [(q' & l'%hs)|].
+         intro eq_nil. destruct l' as (q & mem%sub & l%H3); set_solver.
+         set_solver.
+      ++ intros p (q & mem%sub & l)%hs. eauto.
+    + intros t' μ qs' hle hwqs hneq_nil.
+      eapply (H1 t' μ); eauto. intros p' mem%hwqs. set_solver.
+Qed.
+
+Lemma mx_mem X t :
+  X must_pass_x t
+    -> forall p, p ∈ X
+      -> mustx {[ p ]} t.
+Proof. intros hmx p mem. eapply mx_sub; set_solver. Qed.
+
+Lemma mustx_terminate_unoutcome X t :
+  X must_pass_x t
+    -> outcome t \/ forall p, p ∈ X -> p ⤓.
+Proof.
+  intros hmx.
+  induction hmx.
+  - now left.
+  - right.
+    intros p mem.
+    eapply tstep. intros p' l.
+    edestruct (H {[p']}); [exists p; set_solver| | |]; set_solver.
+Qed.
+
+Lemma mustx_terminate_unoutcome' X (t : T) :
+  X must_pass_x t
+        -> ¬ outcome t -> forall p, p ∈ X -> p ⤓.
+Proof.
+  intros hmx not_happy p mem.
+  dependent induction hmx.
+  + contradiction.
+  + eapply tstep.
+    intros q tr. eapply H; eauto.
+    assert (h1 : lts_tau_set_from_pset_spec1 X {[q]}).
+    exists p. assert (q0 = q);subst. set_solver. split; eauto. eauto.
+    set_solver. set_solver.
+Qed.
+
+Lemma unoutcome_acnv_mu X t t' :
+  X must_pass_x t
+    -> forall μ p, p ∈ X
+        -> t ⟶[μ] t'
+          -> ¬ outcome t -> ¬ outcome t' -> p ⇓ᶜᵒ [μ].
+Proof.
+  intros hmx μ p mem l not_happy not_happy'.
+  dependent induction hmx.
+  - contradiction.
+  - edestruct mustx_terminate_unoutcome as [happy | finish].
+    + eauto with mdb.
+    + contradiction.
+    + edestruct mustx_terminate_unoutcome; eauto with mdb.
+      * contradiction.
+      * eapply cocnv_act.
+        -- eauto.
+        -- intros q w.
+           assert (h1 : cowt_set_from_pset_spec1 X μ {[q]}).
+           { exists p. split; set_solver. }
+           assert (h2 : {[q]} ≠ (∅ : gset P)) by set_solver.
+           set (hm := com t' μ {[ q ]} l h1 h2).
+           destruct (mustx_terminate_unoutcome _ _ hm).
+           +++ contradiction.
+           +++ eapply cocnv_nil. eapply H3. set_solver.
+Qed.
+
+Lemma must_mu_either_outcome_cnv X t t' :
+  X must_pass_x t
+    -> forall μ p, p ∈ X
+        -> t ⟶[μ] t'
+          -> outcome t \/ outcome t' (* ajout par rapport à Input/Output *)
+                       \/ p ⇓ᶜᵒ [μ].
+Proof.
+  intros hmx μ p mem l.
+  destruct (decide (outcome t)); destruct (decide (outcome t')).
+  + left; eauto.
+  + left; eauto.
+  + right; eauto.
+  + right. right. eapply unoutcome_acnv_mu; eauto.
+Qed.
+
+(* to rework , why ?*)
+Lemma mx_sum X X' t : X must_pass_x t
+    -> X' must_pass_x t
+      -> (X ∪ X') must_pass_x t.
+Proof.
+  intros hmx1 hmx2. revert X' hmx2.
+  dependent induction hmx1. eauto with mdb.
+  intros ps2 hmx2.
+  eapply mx_step.
+  - eassumption.
+  - intros p mem.
+    eapply elem_of_union in mem.
+    destruct mem.
+    eapply ex; eassumption.
+    inversion hmx2; subst. contradiction.
+    eapply ex0; eassumption.
+  - intros.
+    set (Y := cowt_tau_set_from_pset X).
+    set (Z := cowt_tau_set_from_pset ps2).
+    assert (X' ⊆ cowt_tau_set_from_pset X ∪ cowt_tau_set_from_pset ps2).
+    { intros q mem. eapply H2 in mem as (q0 & mem & l).
+      eapply elem_of_union in mem. destruct mem.
+      eapply elem_of_union. left. eapply cowt_tau_set_from_pset_ispec; eassumption.
+      eapply elem_of_union. right. eapply cowt_tau_set_from_pset_ispec; eassumption. }
+    eapply lem_dec in H4 as (Y' & Z' & Y_spec' & Z_spec' & eq).
+    remember Y' as Y_'.
+    remember Z' as Z_'.
+    destruct Y_' using set_ind_L.
+    + destruct Z_' using set_ind_L.
+      ++ exfalso.
+         assert (exists p, p ∈ X') as (p & mem).
+         destruct X' using set_ind_L. contradiction.
+         exists x. set_solver.
+         eapply H2 in mem as (p0 & mem & l).
+         eapply elem_of_union in mem. destruct mem.
+         eapply cowt_tau_set_from_pset_ispec in l; set_solver.
+         eapply cowt_tau_set_from_pset_ispec in l; set_solver.
+      ++ assert (Y' = ∅) by set_solver.
+         assert (Z' = X') by set_solver. subst.
+         inversion hmx2; subst. set_solver.
+         eapply pt0. intros t' mem. eapply cowt_tau_set_from_pset_ispec. set_solver. set_solver.
+    + destruct Z_' using set_ind_L.
+      ++ assert (Y' = X') by set_solver.
+         assert (mustx X t) by eauto with mdb.
+         inversion H6; subst. set_solver.
+         eapply pt0. intros t' mem. eapply cowt_tau_set_from_pset_ispec. set_solver. set_solver.
+      ++ subst.
+         replace X' with (({[x]} ∪ X0) ∪ ({[x0]} ∪ X1)) by set_solver.
+         eapply H.
+         +++ intros t' mem. apply cowt_tau_set_from_pset_ispec. set_solver.
+         +++ set_solver.
+         +++ inversion hmx2; subst.
+             ++++ now contradiction nh.
+             ++++ eapply pt0. intros t' mem. eapply cowt_tau_set_from_pset_ispec. set_solver. set_solver.
+  - intros t' l. eapply H0; eauto with mdb.
+    inversion hmx2; subst; eauto with mdb. contradiction.
+  - intros t' μ ps' l ps'_spec neq_nil.
+    destruct (outcome_decidable t'); eauto with mdb.
+    assert (HAX : forall p, p ∈ X -> p ⇓ᶜᵒ [μ]).
+    intros p0 mem0.
+    eapply cocnv_act. edestruct (mustx_terminate_unoutcome X); eauto with mdb.
+    contradiction.
+    intros p' hw. eapply cocnv_nil.
+    edestruct (mustx_terminate_unoutcome {[p']}). eapply com; eauto.
+    intros j memj. eapply elem_of_singleton_1 in memj. subst.
+    exists p0. split; eauto. set_solver.
+    set_solver.
+    set (Y := cowt_s_set_from_pset X μ HAX).
+    assert (HAX2 : forall p, p ∈ ps2 -> p ⇓ᶜᵒ [μ]).
+    intros p0 mem0.
+    eapply cocnv_act. edestruct (mustx_terminate_unoutcome ps2); eauto with mdb.
+    contradiction.
+    intros p' hw. eapply cocnv_nil.
+    edestruct (mustx_terminate_unoutcome {[p']}).
+    inversion hmx2; subst. contradiction. eapply com0; eauto.
+    intros j memj. eapply elem_of_singleton_1 in memj. subst.
+    exists p0. split; eauto. set_solver. set_solver.
+    set (Z := cowt_s_set_from_pset ps2 μ HAX2).
+    assert (ps' ⊆ Y ∪ Z).
+    intros q mem. eapply ps'_spec in mem as (q0 & mem & l').
+    eapply elem_of_union in mem. destruct mem.
+    eapply elem_of_union. left. eapply cowt_s_set_from_pset_ispec; eassumption.
+    eapply elem_of_union. right. eapply cowt_s_set_from_pset_ispec; eassumption.
+    eapply lem_dec in H2 as (Y0 & Z0 & Y_spec0 & Z_spec0 & eq).
+    destruct Y0 using set_ind_L.
+    + destruct Z0 using set_ind_L.
+      ++ exfalso.
+         assert (exists p, p ∈ ps') as (p & mem).
+         destruct ps' using set_ind_L. contradiction.
+         exists x. set_solver.
+         eapply ps'_spec in mem as (p0 & mem & l').
+         eapply elem_of_union in mem.
+         destruct mem; eapply cowt_s_set_from_pset_ispec in l'; set_solver.
+      ++ inversion hmx2; subst.
+         +++ now contradict nh.
+         +++ eapply com0. eassumption. intros t'' mem.
+             eapply (cowt_s_set_from_pset_ispec ps2 μ HAX2).
+             set_solver. set_solver.
+             Unshelve.
+             exact HAX.
+             exact HAX2.
+    + destruct Z0 using set_ind_L.
+      ++ inversion hmx2; subst.
+         +++ now contradict nh.
+         +++ eapply com. eassumption. intros t'' mem.
+             eapply (cowt_s_set_from_pset_ispec X μ HAX).
+             set_solver. set_solver.
+      ++ replace ps' with (({[x]} ∪ X0) ∪ ({[x0]} ∪ X1)) by set_solver.
+         eapply H1; eauto with mdb.
+         +++ intros t'' mem.
+             eapply (cowt_s_set_from_pset_ispec X μ HAX).
+             set_solver.
+         +++ set_solver.
+         +++ inversion hmx2; subst.
+             ++++ now contradict nh.
+             ++++ eapply com0. eassumption.
+                  intros t'' mem.
+                  eapply (cowt_s_set_from_pset_ispec ps2 μ HAX2).
+                  set_solver. set_solver.
+Qed.
+
+Lemma mx_forall X t :
+  X ≠ ∅
+    -> (forall p, p ∈ X -> {[p]} must_pass_x t)
+      -> X must_pass_x t.
+Proof.
+  intros neq_nil hm.
+  induction X using set_ind_L.
+  - set_solver.
+  - destruct (set_choose_or_empty X).
+    + eapply mx_sum.
+      * eapply hm. set_solver.
+      * eapply IHX.
+        -- set_solver.
+        -- intros. eapply hm. set_solver.
+    + assert (X = ∅) by set_solver.
+      rewrite H1, union_empty_r_L. set_solver.
+Qed.
+
+Lemma wt_nil_mx:
+  forall p1 p2 t, {[ p1 ]} must_pass_x t
+    -> p1 ⟹ p2 -> {[ p2 ]} must_pass_x t.
+Proof.
+  intros p1 p2 e hmx wt.
+  dependent induction wt; subst; eauto with mdb.
+  inversion hmx; subst; eauto with mdb.
+  eapply IHwt; eauto with mdb.
+  eapply pt; eauto with mdb.
+  intros p2 mem. replace q with p2 in * by set_solver.
+  exists p; set_solver.
+Qed.
+
+Lemma wt_nil_mx_set (X : gset P) (X' : gset P) t :
+  X must_pass_x t
+    -> wt_set_from_pset_spec1 X [] X' -> X' must_pass_x t.
+Proof.
+  intros hmx wt_tr.
+  destruct (set_choose_or_empty X') as [(x'&mem)|Hemp].
+  - eapply mx_forall.
+    + set_solver.
+    + intros p' mem'.
+      eapply wt_tr in mem' as (p&mem''&w).
+      eapply wt_nil_mx.
+      * eapply mx_mem; eauto.
+      * exact w.
+  - assert (X' = ∅) by set_solver.
+    subst.
+    clear wt_tr.
+    induction hmx.
+    + now eapply mx_now.
+    + eapply mx_step.
+      * eassumption.
+      * intros p mem.
+        inversion mem.
+      * intros Y hY hYne.
+        exfalso. apply hYne.
+        apply leibniz_equiv. intros y. split; [|set_solver].
+        intros mem. eapply hY in mem as (p' & mem_imp & tr). set_solver.
+      * intros t' l.
+        eapply H0; eauto.
+      * intros t' μ Y l hY hYne.
+        exfalso. apply hYne.
+        apply leibniz_equiv. intros y. split; [|set_solver].
+        intros mem. eapply hY in mem as (p' & mem_imp & tr). set_solver.
+Qed.
+
+Lemma co_wt_mu_mx p1 p2 t t' μ :
+  ¬ outcome t -> {[ p1 ]} must_pass_x t
+    -> t ⟶[μ] t' -> p1 ⟹ᶜᵒ{μ} p2 -> {[p2]} must_pass_x t'.
+Proof.
+  intros nh hmx l w.
+  inversion hmx; subst.
+  - contradiction.
+  - eapply com; eauto with mdb. exists p1. set_solver.
+Qed.
+
+Lemma wt_mu_mx_set X X' t t' μ :
+  ¬ outcome t -> X must_pass_x t
+    -> t ⟶[μ] t' -> cowt_set_from_pset_spec1 X μ X' -> X' ≠ ∅ -> X' must_pass_x t'.
+Proof.
+  intros nh hmx l w hne.
+  inversion hmx; subst.
+  - contradiction.
+  - eapply com; eauto.
+Qed.
+
+Lemma must_set_if_must  (p : P) (t : T) : p must_pass t -> {[ p ]} must_pass_x t.
+Proof.
+  intro hm. dependent induction hm.
+  - eauto with mdb.
+  - eapply mx_step.
+    + eassumption.
+    + set_solver.
+    + intros ps' hs hneq_nil.
+      unfold lts_tau_set_from_pset_spec1 in hs.
+      eapply mx_forall; set_solver.
+    + eauto with mdb.
+    + intros e' μ X' hle hws hneq_nil.
+      unfold wt_set_from_pset_spec1 in hws.
+      eapply mx_forall. eassumption.
+      intros.
+      edestruct hws as (p' & mem%elem_of_singleton_1 & w); subst; eauto.
+      inversion w; subst; eauto with mdb.
+      eapply co_wt_mu_mx; eauto with mdb.
+      eapply wt_nil_mx.
+      eapply H1; eauto.
+      eapply cowt_iff_wt_nil; eauto.
+Qed.
+
+Lemma must_if_must_set_helper  (X : gset P) (t : T) :
+  X must_pass_x t
+    -> forall p, p ∈ X
+      -> p must_pass t.
+Proof.
+  intro hm. dependent induction hm.
+  - eauto with mdb.
+  - intros p mem. eapply m_step.
+    + eassumption.
+    + set_solver.
+    + intros p' hl.
+      set (X' := list_to_set (cowt_tau_set  p) : gset P).
+      assert (p' ∈ X').
+      eapply cowt_tau_set_spec , elem_of_list_to_set in hl; eauto.
+      eapply (H X'); eauto.
+      intros p0 mem0%elem_of_list_to_set%cowt_tau_set_spec . set_solver. set_solver.
+    + eauto with mdb.
+    + intros p' e' μ μ' duo hlp hle.
+      assert (Finite (dsig (λ q : P, dual μ μ' ∧ p ⟶[μ] q))).
+      { unfold dsig.
+        eapply (in_list_finite (map proj1_sig (enum (dsig (fun q => exists α', dual α' μ' /\ p ⟶[α'] q))))).
+        intros q Hq. eapply bool_decide_unpack in Hq.
+        eapply list_elem_of_fmap.
+        exists (dexist q (ex_intro _ μ (conj duo (proj2 Hq)))).
+        split; [reflexivity | eapply elem_of_enum]. }
+      set (X' := list_to_set (
+                     map proj1_sig (enum $ dsig (fun q => dual μ μ' /\ p ⟶[μ] q))
+                   ) : gset P).
+      assert (p' ∈ X').
+      eapply elem_of_list_to_set, list_elem_of_fmap; eauto.
+      assert (hlp' : dual μ μ' /\ p ⟶[μ] p'). eexists; eauto.
+      exists (dexist p' hlp'). split. eauto. eapply elem_of_enum.
+      eapply (H1 e' μ' X'). eassumption.
+      intros p0 mem0%elem_of_list_to_set.
+      eapply list_elem_of_fmap in mem0 as ((r & l) & eq & mem'). subst.
+      exists p. split; eauto.
+      eapply cowt_act. eauto.
+      assert (mem'' : dual μ μ' /\ p ⟶[μ] r ).
+      { eapply bool_decide_unpack. eauto. }
+      destruct mem'' as (duo'' & tr''). exact tr''.
+      eapply cowt_nil. set_solver. set_solver.
+Qed.
+
+Lemma must_if_must_set  (p : P) (t : T) :
+  {[ p ]} must_pass_x t
+    -> p must_pass t.
+Proof. intros. eapply must_if_must_set_helper; set_solver. Qed.
+
+Lemma must_set_iff_must  (p : P) (t : T) :
+  p must_pass t <-> mustx {[ p ]} t.
+Proof. split; [eapply must_set_if_must | eapply must_if_must_set]. Qed.
+
+Lemma must_set_for_all  (X : gset P) (t : T) :
+  X ≠ ∅
+    -> (forall p, p ∈ X -> p must_pass t)
+      -> X must_pass_x t.
+Proof.
+  intros xneq_nil hm.
+  destruct (outcome_decidable t).
+  - now eapply mx_now.
+  - eapply mx_step.
+    + eassumption.
+    + intros p h%hm. inversion h. contradiction. eassumption.
+    + intros X' xspec' xneq_nil'.
+      eapply mx_forall. eassumption.
+      intros p' (p0 & mem%hm & hl)%xspec'. eapply must_set_iff_must.
+      inversion mem; eauto with mdb.
+    + intros t' hl.
+      eapply mx_forall. eassumption.
+      intros p' mem%hm. eapply must_set_iff_must.
+      inversion mem; eauto with mdb. contradiction.
+    + intros t' μ X' hle xspec' xneq_nil'.
+      eapply mx_forall. eassumption.
+      intros p' (p0 & h%hm & hl)%xspec'. eapply must_set_iff_must.
+      eapply cowt_to_wt_dual in hl as (s' & duo & wk_tr).
+      inversion duo;subst. symmetry in H1.
+      eapply must_preserved_by_wt_synch_if_notoutcome ; eauto.
+      inversion H3;subst;eauto.
+Qed.
+
+Lemma must_set_iff_must_for_all  (X : gset P) (t : T) :
+  X ≠ ∅ -> (forall p, p ∈ X -> p must_pass t) <-> X must_pass_x t.
+Proof.
+  intros.
+  split. now eapply must_set_for_all.
+  now eapply must_if_must_set_helper.
+Qed.
+
+End Must_for_sets.
+
+(** ** Contextual preorder for sets *)
+
+Section Must_preorder_for_sets.
+Context `{EA : !ExtAction A}.
+Context `{gLtsT : !gLtsEq T EA}.
+Context `{TP : @Testing_Predicate T A EA outcome _}.
+
+Context `{gLtsP : @gLts P A EA, !coFiniteImagegLts P A}.
+Context `{HinterP : !Prop_of_Inter P T A dual}.
+Context `{gLtsQ : @gLts Q A EA, !coFiniteImagegLts Q A}.
+Context `{HinterQ : !Prop_of_Inter Q T A dual}.
+
+Definition ctx_pre__x
+  (X : gset P) (Y : gset Q)
+  := forall (t : T), X must_pass_x t -> Y must_pass_x t.
+Notation "X ⊑ₛₑₜ_ₘᵤₛₜᵢ Y" := (ctx_pre__x X Y) (at level 70).
+Notation "X ⋢ₛₑₜ_ₘᵤₛₜᵢ Y" := (¬ ctx_pre X Y) (at level 70).
+
+Lemma set_must_union_right
+  (X : gset P) (Y Y' : gset Q) : X ⊑ₛₑₜ_ₘᵤₛₜᵢ Y -> X ⊑ₛₑₜ_ₘᵤₛₜᵢ Y' ->  X ⊑ₛₑₜ_ₘᵤₛₜᵢ (Y ∪ Y').
+Proof.
+  intros Hyp1 Hyp2.
+  intros t h_must.
+  - eapply mx_sum.
+    + eapply Hyp1; eauto.
+    + eapply Hyp2; eauto.
+Qed.
+
+Lemma set_must_empty (X : gset P) : X ⊑ₛₑₜ_ₘᵤₛₜᵢ ∅.
+Proof.
+  intros t h_must.
+  induction h_must.
+  + now eapply mx_now.
+  + eapply mx_step;eauto.
+    * intros p mem. inversion mem.
+    * intros. destruct X' using set_ind_L.
+      - exfalso. eapply H3;eauto.
+      - assert (x ∈ {[x]} ∪ X0) as mem'' by set_solver.
+        eapply H2 in mem'' as (p' & mem_imp & tr). inversion mem_imp.
+    * intros. destruct X' using set_ind_L.
+      - exfalso. eapply H4;eauto.
+      - assert (x ∈ {[x]} ∪ X0) as mem'' by set_solver.
+        eapply H3 in mem'' as (p' & mem_imp & tr). inversion mem_imp.
+Qed.
+
+Lemma set_must_union_left_rev
+  (X : gset P) (Y Y' : gset Q) : X ⊑ₛₑₜ_ₘᵤₛₜᵢ (Y ∪ Y') -> X ⊑ₛₑₜ_ₘᵤₛₜᵢ Y.
+Proof.
+  intros Hyp t h_must.
+  induction Y using set_ind_L.
+  - eapply set_must_empty;eauto.
+  - eapply Hyp in h_must. eapply must_set_for_all. set_solver.
+    intros. eapply must_if_must_set_helper in h_must.
+    set_solver. set_solver.
+Qed.
+
+Lemma set_must_union_right_rev
+  (X : gset P) (Y Y' : gset Q) : X ⊑ₛₑₜ_ₘᵤₛₜᵢ (Y ∪ Y') -> X ⊑ₛₑₜ_ₘᵤₛₜᵢ Y'.
+Proof.
+  intros Hyp t h_must.
+  induction Y' using set_ind_L.
+  - eapply set_must_empty;eauto.
+  - eapply Hyp in h_must. eapply must_set_for_all. set_solver.
+    intros. eapply must_if_must_set_helper in h_must.
+    set_solver. set_solver.
+Qed.
+
+Lemma set_must_sub
+  (X : gset P) (Y : gset Q) : X ⊑ₛₑₜ_ₘᵤₛₜᵢ Y -> forall Y', Y' ⊆ Y ->  X ⊑ₛₑₜ_ₘᵤₛₜᵢ Y'.
+Proof.
+  intros Hyp Y' sub t h_must.
+  destruct Y' using set_ind_L.
+  + eapply set_must_empty;eauto.
+  + eapply Hyp in h_must. eapply must_set_for_all. set_solver.
+    intros. eapply must_if_must_set_helper in h_must.
+    set_solver. set_solver.
+Qed.
+
+(** ** Equivalence between the must preorder and the must preorder on sets *)
+Lemma must_set_singleton_iff (p : P) (q : Q) :
+  p ⊑ₘᵤₛₜᵢ q <-> {[ p ]} ⊑ₛₑₜ_ₘᵤₛₜᵢ {[ q ]}.
+Proof.
+  split.
+  - intro must_hyp. intros t Hyp_set_p.
+    eapply must_if_must_set in Hyp_set_p.
+    eapply must_hyp in Hyp_set_p as Hyp_set_q.
+    eapply must_set_if_must in Hyp_set_q. exact Hyp_set_q.
+  - intro set_must_hyp. intros t Hyp_p.
+    eapply must_set_if_must in Hyp_p.
+    eapply set_must_hyp in Hyp_p as Hyp_q.
+    eapply must_if_must_set in Hyp_q. exact Hyp_q.
+Qed.
+
+End Must_preorder_for_sets.
+
+#[global] Hint Unfold ctx_pre__x : mdb.
+Notation "X ⊑ₛₑₜ_ₘᵤₛₜᵢ Y" := (ctx_pre__x X Y) (at level 70).
+Notation "X ⋢ₛₑₜ_ₘᵤₛₜᵢ Y" := (¬ ctx_pre X Y) (at level 70).
+
+(* The relation ⊑ₛₑₜ_ₘᵤₛₜᵢ is reflexive *)
+#[global] Instance set_must_refl
+  `{EA : !ExtAction A} `{gLtsT : !gLtsEq T EA} `{TP : @Testing_Predicate T A EA outcome _}
+  `{gLtsP : @gLts P A EA, !coFiniteImagegLts P A} {Hinter : @Prop_of_Inter P T A dual EA gLtsP _} : Reflexive ctx_pre__x.
+Proof. intros X t h_must. eauto. Qed.
+
+(* The relation ⊑ₛₑₜ_ₘᵤₛₜᵢ is transitive *)
+#[global] Instance set_must_transitive
+  `{EA : !ExtAction A} `{gLtsT : !gLtsEq T EA} `{TP : @Testing_Predicate T A EA outcome _}
+  `{gLtsP : @gLts P A EA, !coFiniteImagegLts P A} {Hinter : @Prop_of_Inter P T A dual EA gLtsP _} : Transitive ctx_pre__x.
+Proof.
+  intros X Y Z hcgr1 hcgr2. intros t h_must.
+  eapply hcgr2. eapply hcgr1; eauto.
+Qed.
+
+(* The relation ⊑ₛₑₜ_ₘᵤₛₜᵢ is a preorder *)
+#[global] Instance set_must_x_preorder
+  `{EA : !ExtAction A} `{gLtsT : !gLtsEq T EA} `{TP : @Testing_Predicate T A EA outcome _}
+  `{gLtsP : @gLts P A EA, !coFiniteImagegLts P A} {Hinter : @Prop_of_Inter P T A dual EA gLtsP _} : PreOrder ctx_pre__x.
+Proof.
+  split.
+  + exact set_must_refl.
+  + exact set_must_transitive.
+Qed.
+
+Notation "X ≂ₛₑₜ_ₘᵤₛₜᵢ Y" := (Y ⊑ₛₑₜ_ₘᵤₛₜᵢ X /\ X ⊑ₛₑₜ_ₘᵤₛₜᵢ Y) (at level 70).
+
+(** ** [mustx_alt] — the one piece of [mustx]'s apparatus that *does* need a
+    co-variant: its [com] case is where the (map-[coₜ]-free) design pays off.
+    Mirrors [mustx]'s own two-label ([wt_set_from_pset_spec1 X [μ1] X'] +
+    [dual μ1 μ2]) style, but with a single [μ] via [cowt_set_from_pset_spec1]
+    (itself just [wt_set_from_pset_spec1]'s pattern rebuilt on [⟹ᶜᵒ]) — this
+    keeps the bridge to [mustx] a direct, per-element one (no need to route
+    through [toSET]'s "exact union" semantics, which only obscures the
+    already-immediate correspondence). The bridge itself needs [dual]'s
+    global uniqueness ([unique_nb], unrestricted to non-blocking actions
+    despite the name — see [gLts.v]) once, to turn the existential dual
+    witness [cowt_set_from_pset_spec1] hides back into the single fixed label
+    [wt_set_from_pset_spec1] needs; this is a legitimate external use of a
+    real class law, unlike baking [unique_nb]/canonical [co] into [cowt]'s
+    own definition (which stays fully dual-relational, per
+    [[co_trace_files_dual_bridge]]). *)
+
+(* [mustx_alt_co]'s own [pt] field uses the set LTS ([toSET], [X ⟶ X'] on
+   [gset P]) — the piece the header comment (top of file) calls out as the
+   one place [mustx]'s apparatus structurally needs [FiniteImagegLts] for
+   [SetLTSConstruction.toSET]. *)
+(*
+Inductive mustx_alt_co `{EA : !ExtAction A} `{gLtsT : !gLtsEq T EA} `{TP : @Testing_Predicate T A EA outcome _}
+  `{gLtsP : @gLts P A EA, !FiniteImagegLts P A} {Hinter : @Prop_of_Inter P T A dual EA gLtsP _}
+  (X : gset P) (t : T) : Prop :=
+| mx_now_alt_co (hh : outcome t) : mustx_alt_co X t
+| mx_step_alt_co
+    (nh : ¬ outcome t)
+    (ex : forall (p : P), p ∈ X -> ∃ p', inter_step (p, t) τ p')
+    (pt : forall X',
+        X ⟶ X' ->
+        mustx_alt_co X' t)
+    (et : forall (t' : T), t ⟶ t' -> mustx_alt_co X t')
+    (com : forall (t' : T) μ (X' : gset P),
+        t ⟶[μ] t' ->
+        X ⟹ᶜᵒ{μ} X' ->
+        mustx_alt_co X' t')
+  : mustx_alt_co X t.
+
+#[global] Hint Constructors mustx_alt_co:mdb.
+Global Notation "X 'must_alt_pass_x_co' t" := (mustx_alt_co X t) (at level 70).
+*)
+
+(* [mustx_iff_mustx_alt_co] bridges [mustx] to [mustx_alt_co] — depends on
+   the (now commented-out) set-LTS-based [mustx_alt_co]. *)
+(*
+Section MustxIffMustxAltCo.
+
+(* This bridge lemma needs [mustx] (⇒ [coFiniteImagegLts P A]) and
+   [mustx_alt_co] (⇒ [FiniteImagegLts P A], for its toSET-based [pt] case)
+   simultaneously on the *same* [X : gset P] — so the two [Countable P]
+   sources must be the same term, not two independent postulates (see
+   [[bang_vs_bare_class_binder]]-style clash risk). [coFiniteImagegLts P A]
+   is taken as primary and [FiniteImagegLts P A] is derived locally via
+   [FiniteImagegLts_of_coFiniteImagegLts], sharing the countable field by
+   construction. Any caller supplying the *same* [coFiniteImagegLts P A]
+   term for both this lemma and [mustx_alt_co]'s own use gets a matching
+   derived instance automatically (it's a pure function of that term). *)
+Context `{EA : !ExtAction A}.
+Context `{gLtsT : !gLtsEq T EA}.
+Context `{TP : @Testing_Predicate T A EA outcome _}.
+Context `{gLtsP : @gLts P A EA, !coFiniteImagegLts P A}.
+#[local] Instance MustxIffMustxAltCo_FI_PP : FiniteImagegLts P A 
+    := FiniteImagegLts_of_coFiniteImagegLts _.
+Context `{Hinter : @Prop_of_Inter P T A dual EA gLtsP _}.
+
+Lemma mustx_iff_mustx_alt_co
+  (X : gset P) (t : T) :
+  X must_pass_x t <-> X must_alt_pass_x_co t.
+Proof.
+  split.
+  - intro hmx. dependent induction hmx; eauto.
+    + constructor ;eauto.
+    + eapply mx_step_alt_co; eauto.
+      * intros. destruct H2;eauto. subst.
+        assert (lts_tau_set_from_pset_spec1 X (cowt_tau_set_from_pset X)).
+        { eapply cowt_tau_set_from_pset_ispec. }
+        eauto.
+      * intros t' μ X' hle hws.
+        eapply (H1 t' (co μ) μ X'); eauto.
+        -- symmetry. exact (proj2_sig (exists_dual μ)).
+        -- intros q mem. eapply hws in mem as (p & mem & w).
+           eapply cowt_to_wt_dual in w as (s' & hf & w').
+           assert (Hy : exists y, s' = [y] /\ dual μ y).
+           { inversion hf as [| ? y ? ? duo hf2]; subst. inversion hf2; subst. eauto. }
+           destruct Hy as (y & -> & duo).
+           assert (y = co μ) by (eapply unique_nb; exact duo).
+           subst. exists p. eauto.
+  - intro hmx. dependent induction hmx; eauto.
+    + constructor ;eauto.
+    + eapply mx_step; eauto.
+      * intros. assert (X' ⊆ cowt_tau_set_from_pset X).
+        { intros p' mem'. eapply H2 in mem' as (p & mem & tr).
+          eapply cowt_tau_set_from_pset_ispec;eauto. }
+        assert (cowt_tau_set_from_pset X  ≠ ∅ ) by set_solver.
+        assert (X ⟶ cowt_tau_set_from_pset X).
+        { split ;eauto. }
+        eapply H in H6. eapply mx_sub;eauto.
+      * intros t' μ1 μ2 X' duo hle hws hneq.
+        eapply (H1 t' μ2 X'); eauto.
+        intros q mem. eapply hws in mem as (p & mem & w).
+        exists p. split; eauto. eapply wt_to_cowt_dual with (s' := [μ1]); eauto.
+        constructor; [symmetry; exact duo | constructor].
+Qed.
+
+End MustxIffMustxAltCo.
+*)
+
+(** ** Condition on convergence *)
+
+Definition bhv_pre_co_cond1__x `{gLtsP : @gLts P A EA, !Countable P}
+  `{gLtsQ : @gLts Q A EA, !Countable Q}
+  (X : gset P) (Y : gset Q) :=
+  forall s, (forall p, p ∈ X -> p ⇓ᶜᵒ s) -> (forall q, q ∈ Y -> q ⇓ᶜᵒ s).
+
+Global Notation "X ₁≼꜀ₒ₋ₛₑₜ_ₐₛ Y" := (bhv_pre_co_cond1__x X Y) (at level 70).
+
+(** ** Condition on acceptance sets *)
+
+Definition bhv_pre_co_cond2__x
+  `{gLtsP : @gLts P A EA, !Countable P}
+  `{gLtsQ : @gLts Q A EA, !Countable Q}
+  `{gLtsT : @gLtsEq T A EA}
+  `{AbsPT : @AbsAction P T FinA PreAct A EA Φ 𝝳P _ _}
+  `{AbsQT : @AbsAction Q T FinA PreAct A EA Φ 𝝳Q _ _}
+  (X : gset P) (Y : gset Q) :=
+  forall q s q', q ∈ Y ->
+    q ⟹ᶜᵒ[s] q' -> q' ↛ ->
+    (forall p, p ∈ X -> p ⇓ᶜᵒ s) ->
+    exists p, p ∈ X /\ exists p', p ⟹ᶜᵒ[s] p' /\ p' ↛ /\ (⌈ (𝝳P ∘ Φ) ⌉ (coR p') ⊆ ⌈ (𝝳Q ∘ Φ) ⌉ (coR q')).
+
+Global Notation "X ₂≼꜀ₒ₋ₛₑₜ_ₐₛ Y" := (bhv_pre_co_cond2__x X Y) (at level 70).
+
+(** ** Alternative preorder on sets *)
+
+Definition bhv_pre_co__x
+  `{gLtsP : @gLts P A EA, !Countable P}
+  `{gLtsQ : @gLts Q A EA, !Countable Q}
+  `{gLtsT : @gLtsEq T A EA}
+  `{AbsPT : @AbsAction P T FinA PreAct A EA Φ 𝝳P _ _}
+  `{AbsQT : @AbsAction Q T FinA PreAct A EA Φ 𝝳Q _ _}
+    (X : gset P) (Y : gset Q) :=
+      (X ₁≼꜀ₒ₋ₛₑₜ_ₐₛ Y /\ X ₂≼꜀ₒ₋ₛₑₜ_ₐₛ Y).
+
+Global Notation "X ≼꜀ₒ₋ₛₑₜ_ₐₛ Y" := (bhv_pre_co__x X Y) (at level 70).
+
+(** ** Acceptance-set preorder properties, co variant
+
+    Mirrors [Acceptance_Set_preorder_for_sets] (Soundness.v), scoped down to
+    the lemmas [soundnessx_co] actually needs. No [FiniteImagegLts P/Q A]
+    anywhere: every lemma body here only ever needs a *bare* [Countable
+    P]/[Countable Q] for the [cowt_set_from_pset_spec1/spec2] obligations —
+    not even [coFiniteImagegLts] is needed here (in particular
+    [reverse_trace_inclusion_co]'s witness set is built directly as a
+    singleton [{[p']}] from [bhv_pre_co_cond2__x]'s own match, sidestepping
+    the constructive [cowt_s_set_from_pset] entirely). Kept on bare
+    [!Countable P/Q] (matching [bhv_pre_co_cond1__x]/[bhv_pre_co_cond2__x]/
+    [bhv_pre_co__x] above) rather than [coFiniteImagegLts P/Q A]: since
+    [coFiniteImagegLts]'s own [Countable] field is declared with [::]
+    (a genuine sub-instance projection, see [coFiniteImage.v]), any
+    [Countable P] resolved here from a caller's ambient [coFiniteImagegLts
+    P A] (e.g. [SoundnessAS_co]'s own [soundnessx_co]) is *the same term*
+    by construction — no clash risk, unlike two independently-postulated
+    [Countable P] siblings would have. *)
+
+Section Acceptance_Set_preorder_for_sets_co.
+
+Context `{EA : !ExtAction A}.
+Context `{gLtsEqT : !gLtsEq T EA}.
+
+Context `{gLtsP : @gLts P A EA, !Countable P}.
+Context `{AbsPT : @AbsAction P T FinA PreAct A EA Φ 𝝳P _ _}.
+
+Context `{gLtsQ : @gLts Q A EA, !Countable Q}.
+Context `{AbsQT : @AbsAction Q T FinA PreAct A EA Φ 𝝳Q _ _}.
+
+Lemma alt_set_singleton_iff_co
+  (p : P) (q : Q) : ({[ p ]} : gset P) ≼꜀ₒ₋ₛₑₜ_ₐₛ ({[ q ]} : gset Q) <->  p ≼꜀ₒ₋ₐₛ q.
+Proof.
+  split.
+  - intros (hbhv1 & hbhv2). split.
+    + intros s mem. eapply hbhv1. set_solver. set_solver.
+    + intros s q' w st hcnv. edestruct hbhv2; set_solver.
+  - intros (h1 & h2). split.
+    + intros s mem. intros q' mem'.
+      assert (q' = q) by set_solver. subst. eapply h1. set_solver.
+    + intros q' s q'' w st hcnv.
+      assert (q' = q) by set_solver. subst. intros.
+      exists p. edestruct h2 ; set_solver.
+Qed.
+
+Lemma bhvleqone_preserved_by_reduction_co
+  (X : gset P) (Y Y' : gset Q) :
+  X ₁≼꜀ₒ₋ₛₑₜ_ₐₛ Y -> lts_tau_set_from_pset_spec1 Y Y' -> X ₁≼꜀ₒ₋ₛₑₜ_ₐₛ Y'.
+Proof.
+  intros halt1 l s mem.
+  intros. eapply l in H as (q' & mem' & tr').
+  eapply cocnv_preserved_by_lts_tau; eauto.
+Qed.
+
+(* Uses the set LTS ([toSET], [Y ⟶ Y'] on [gset Q]). *)
+(*
+Lemma bhvleqone_preserved_by_reduction_lts_co
+  (X : gset P) (Y Y' : gset Q) :
+  X ₁≼꜀ₒ₋ₛₑₜ_ₐₛ Y -> Y ⟶ Y' -> X ₁≼꜀ₒ₋ₛₑₜ_ₐₛ Y'.
+Proof.
+  intros; eapply bhvleqone_preserved_by_reduction_co;eauto.
+  destruct H0. subst. eapply cowt_tau_set_from_pset_ispec.
+Qed.
+*)
+
+Lemma bhvx_preserved_by_reductions_co
+  (X : gset P) (Y Y' : gset Q) : wt_set_from_pset_spec1 Y [] Y' -> X ≼꜀ₒ₋ₛₑₜ_ₐₛ Y -> X ≼꜀ₒ₋ₛₑₜ_ₐₛ Y'.
+Proof.
+  intros l (halt1 & halt2).
+  split.
+  - intros s mem. intros.
+    eapply l in H as (q' & tr & mem').
+    eapply cocnv_preserved_by_cowt_nil; eauto.
+    eapply cowt_iff_wt_nil; eauto.
+  - intros q' s q'' mem w st hcnv.
+    eapply l in mem as (q & mem2 & tr).
+    destruct (halt2 q s q'') as (p' & mem' & p'' & hw & hst); eauto with mdb.
+    eapply cowt_push_nil_left;eauto. eapply cowt_iff_wt_nil; eauto.
+Qed.
+
+Lemma bhvx_preserved_by_reduction_co
+  (X : gset P) (Y Y' : gset Q) : lts_tau_set_from_pset_spec1 Y Y' -> X ≼꜀ₒ₋ₛₑₜ_ₐₛ Y -> X ≼꜀ₒ₋ₛₑₜ_ₐₛ Y'.
+Proof.
+  intros l (halt1 & halt2).
+  eapply bhvx_preserved_by_reductions_co;eauto.
+  intros q' mem'. eapply l in mem' as (q'' & mem'' & wt_tr'').
+  exists q''. split; eauto. eapply lts_to_wt_tau;eauto. split ;eauto.
+Qed.
+
+(* Uses the set LTS ([toSET], [Y ⟶ Y'] on [gset Q]). *)
+(*
+Lemma bhvx_preserved_by_reduction_lts_co
+  (X : gset P) (Y Y' : gset Q) : Y ⟶ Y' -> X ≼꜀ₒ₋ₛₑₜ_ₐₛ Y -> X ≼꜀ₒ₋ₛₑₜ_ₐₛ Y'.
+Proof.
+  intros. eapply bhvx_preserved_by_reductions_co;eauto.
+  destruct H. subst. intros q'' mem''.
+  destruct (cowt_tau_set_from_pset_ispec Y) as (Hyp1 & Hyp2).
+  eapply Hyp1 in mem'' as (q & mem & wt_tr).
+  exists q. split ;eauto. eapply lts_to_wt_tau;eauto.
+Qed.
+*)
+
+Lemma bhvleqone_preserved_by_external_action_co
+  (X X' : gset P) μ (Y Y' : gset Q) (htp : forall p, p ∈ X -> terminate p) :
+  X ₁≼꜀ₒ₋ₛₑₜ_ₐₛ Y -> cowt_set_from_pset_spec X μ X'  -> cowt_set_from_pset_spec1 Y μ Y' -> X' ₁≼꜀ₒ₋ₛₑₜ_ₐₛ Y'.
+Proof.
+  intros hleq hws l s hcnv. intros.
+  eapply l in H as (q' & mem' & wk_tr).
+  eapply cocnv_preserved_by_cowt_act;eauto.
+  eapply hleq.
+  intros p mem''. eapply cocnv_act.
+  + eapply htp; eauto.
+  + intros. eapply hcnv, hws; eassumption.
+  + exact mem'.
+Qed.
+
+Lemma bhvx_preserved_by_external_action_co
+  (X X' : gset P) μ (Y Y' : gset Q) (htp : forall p, p ∈ X -> terminate p) :
+  cowt_set_from_pset_spec1 Y μ Y'
+    -> cowt_set_from_pset_spec X μ X'
+      -> X ≼꜀ₒ₋ₛₑₜ_ₐₛ Y
+        -> X' ≼꜀ₒ₋ₛₑₜ_ₐₛ Y'.
+Proof.
+  intros lts__q ps1_spec (halt1 & halt2). split.
+  - eapply bhvleqone_preserved_by_external_action_co; eauto.
+  - intros q s q0 mem wt st hcnv. assert (cowt_set_from_pset_spec1 Y μ Y') as tr'';eauto.
+    eapply tr'' in mem as (q' & mem' & tr_ext);eauto.
+    edestruct (halt2 q' (μ :: s) q0) as (t & mem'' & p0 & p1 & wta__t & sub); eauto with mdb.
+    + eapply cowt_push_left; eauto.
+    + intros p'' mem1. eapply cocnv_act.
+      * eapply htp; eauto.
+      * intros q1 wk_tr. destruct ps1_spec as (ps1s1 & ps1s2).
+        eapply ps1s2 in wk_tr; eauto.
+    + eapply cowt_pop in p1 as (r & w1 & w2).
+      exists r. repeat split. destruct ps1_spec as (ps1s1 & ps1s2). eapply ps1s2; eassumption. eauto.
+Qed.
+
+Lemma reverse_trace_inclusion_co
+  (X : gset P) (Y Y' : gset Q) μ
+  : X ≼꜀ₒ₋ₛₑₜ_ₐₛ Y -> (forall p, p ∈ X -> p ⇓ᶜᵒ [μ]) ->
+    cowt_set_from_pset_spec1 Y μ Y' -> Y' ≠ ∅ ->
+    exists X', cowt_set_from_pset_spec1 X μ X' /\ X' ≠ ∅.
+Proof.
+  intros (h1 & h2) hcnv hl not_empty.
+  destruct (set_choose_L Y' not_empty) as (q0 & mem0).
+  eapply hl in mem0 as (q & mem & w).
+  assert (hq0 : q0 ⤓).
+  { eapply equiv_cotermination.
+    eapply cocnv_preserved_by_cowt_act.
+    - eapply h1; eauto.
+    - exact w. }
+  destruct (terminate_then_wt_refuses q0 hq0) as (q0' & wq0 & stq0).
+  assert (w' : q ⟹ᶜᵒ[[μ]] q0').
+  { eapply cowt_push_nil_right; eauto. eapply cowt_iff_wt_nil; eauto. }
+  edestruct (h2 q [μ] q0' mem w' stq0 hcnv) as (p & memp & p' & wp & stp & sub).
+  exists ({[ p' ]}).
+  split.
+  - intros q1 mem1. exists p. split; eauto. assert (q1 = p') by set_solver. subst. exact wp.
+  - set_solver.
+Qed.
+
+End Acceptance_Set_preorder_for_sets_co.
+
+(** ** Communication-enabling property, co variant
+
+    [communication_enabled] itself needs no co-analogue: it reasons purely
+    about single LTS steps ([⟶]) and the [dual]/[coR]/[Φ]/[𝝳] apparatus,
+    none of which is co- or plain-specific — copied verbatim, exactly like
+    [mustx]. Keeps [𝝳] SHARED between P and Q (not split into 𝝳P/𝝳Q): a
+    prior finding in this session showed the proof genuinely needs the two
+    sides to share one delta.
+
+    Stated with an explicit [dual μ1 μ2] rather than a hardcoded [co μ] on
+    either side — [cn_enabled]/[coR] are already fully general (take/give
+    an arbitrary dual witness, not the canonical one specifically), so the
+    whole proof goes through without ever invoking [unique_nb]/[co]:
+    [dual]'s witnesses are used exactly as given, never pinned down to the
+    canonical one. Diverges from [communication_enabled] (the original,
+    plain, `co`-hardcoded version) for this reason; the caller
+    ([unoutcome_must_st_nleqx_co]) correspondingly drops the
+    [assert (μ1 = co μ2)] step it would otherwise need. *)
+
+Section Properties_for_soundness_co.
+
+Context `{EA : !ExtAction A}.
+Context `{gLtsT : !gLtsEq T EA}.
+Context `{TP : @Testing_Predicate T A EA outcome _}.
+
+Context `{gLtsP : @gLts P A EA}.
+Context `{HinterP : !Prop_of_Inter P T A dual}.
+Context `{gLtsQ : @gLts Q A EA}.
+Context `{HinterQ : !Prop_of_Inter Q T A dual}.
+
+Context `{AbsPT : @AbsAction P T FinA PreAct A EA Φ 𝝳 _ _}.
+Context `{AbsQT : @AbsAction Q T FinA PreAct A EA Φ 𝝳 _ _}.
+
+Context `{!gLtsCNenabled Q A}.
+
+Lemma communication_enabled_co (p : P) p' (q : Q) (t : T) t' μ1 μ2 :
+      dual μ1 μ2 -> p ⟶[μ1] p' -> t ⟶[μ2] t' -> ⌈ (𝝳 ∘ Φ) ⌉ (coR p) ⊆ ⌈ (𝝳 ∘ Φ) ⌉ (coR q)
+        -> exists ν1 ν2 q' t'', dual ν1 ν2 /\ q ⟶[ν1] q' /\ t ⟶[ν2] t''.
+Proof.
+  intros duo tr tr_co sub.
+  destruct (decide (non_blocking μ2)) as [nb | not_nb].
+  + eapply (cn_enabled q μ2 μ1) in nb as (q' & tr'); [| symmetry; exact duo].
+    exists μ1, μ2, q', t'. eauto.
+  + assert (μ2 ∈ coR p) as some_co_action_of_p.
+    { exists μ1. repeat split; eauto.
+      eapply lts_refuses_spec2;eauto. }
+    eapply (map_gamma_of_action (𝝳 ∘ Φ)) in some_co_action_of_p as mem.
+    eapply sub in mem. destruct mem as (μ' & mem & eq).
+    eapply (map_gamma_of_action Φ) in mem as eq'. symmetry in eq.
+    eapply (abstraction_prog_spec q) in eq' ;eauto.
+    2:{ destruct mem as (ν & hmem & hdual & hblock). eauto. }
+    destruct eq' as (μ'' & mem' & eq'). destruct mem' as (μ''' & tr' & duo2 & b).
+    assert (μ'' ∈ R t) as Tr_Test.
+    { eapply abstraction_test_spec in eq';eauto. apply lts_refuses_spec2. eauto. }
+    eapply lts_refuses_spec1 in Tr_Test as (t'' & Tr'').
+    eapply lts_refuses_spec1 in tr' as (q' & tr').
+    exists μ''', μ'', q', t''. eauto.
+Qed.
+
+End Properties_for_soundness_co.
+
+(** ** Soundness for sets, co variant *)
+
+Section SoundnessAS_co.
+
+Context `{EA : !ExtAction A}.
+Context `{gLtsEqT : !gLtsEq T EA}.
+Context `{TP : @Testing_Predicate T A EA outcome _}.
+
+(* [mustx] is used on both sides ([X must_pass_x t] directly, and
+   [Y must_pass_x t] via [mustx_iff_mustx_alt_co]/[mustx_alt_co] inside
+   [soundnessx_co]) — needs only [coFiniteImagegLts]. No [FiniteImagegLts]
+   instance (local or global) is needed in this section any more: the only
+   lemmas here that ever needed it ([unoutcome_must_st_nleqx_co],
+   [stability_nbhvleqtwo_co], via [bhv_pre_co_cond2__x]) are unused now
+   that their only caller ([soundnessx_co]) is commented out (set-LTS-based
+   — see that comment), so they're commented out too, below. *)
+Context `{gLtsP : @gLts P A EA, !coFiniteImagegLts P A}.
+Context `{!Prop_of_Inter P T A dual}.
+Context `{gLtsQ : @gLts Q A EA, !coFiniteImagegLts Q A, !gLtsCNenabled Q A}.
+Context `{!Prop_of_Inter Q T A dual}.
+
+Context `{AbsPT : @AbsAction P T FinA PreAct A EA Φ 𝝳 _ _}.
+Context `{AbsQT : @AbsAction Q T FinA PreAct A EA Φ 𝝳 _ _}.
+
+(* Both need [FiniteImagegLts P/Q A] (via [bhv_pre_co_cond2__x]) and are
+   unused now that their only caller, [soundnessx_co], is commented out. *)
+
+Lemma unoutcome_must_st_nleqx_co (X : gset P) (Y : gset Q) (t : T):
+  ¬ outcome t
+    -> X must_pass_x t
+      -> (∃ q, q ∈ Y /\ (q, t) ↛)
+        -> ¬ X ₂≼꜀ₒ₋ₛₑₜ_ₐₛ Y.
+Proof.
+  intros not_happy all_must (q & mem' & refuses_tau_q) hbhv2.
+  assert (q ↛) as stable_q.
+  { destruct (lts_refuses_decidable q τ) as [refuses_q | not_refuses_q].
+    - exact refuses_q.
+    - exfalso. eapply lts_refuses_spec1 in not_refuses_q as (q' & l).
+      eapply (lts_refuses_spec2 (q ▷ t)); eauto. exists (q' ▷ t). eapply ParLeft. exact l. }
+  assert (htX : ∀ p : P, p ∈ X → p ⇓ᶜᵒ []).
+  { destruct (mustx_terminate_unoutcome X t all_must) as [|htps]; eauto with mdb. contradiction. }
+  assert (w0 : q ⟹ᶜᵒ[[]] q). { eapply cowt_iff_wt_nil. eauto with mdb. }
+  destruct (hbhv2 q [] q mem' w0 stable_q htX) as (p & mem & p' & wp & stp' & sub).
+  assert (mustx {[ p' ]} t) as must_p'.
+  { eapply (wt_nil_mx p). eapply (mx_sub X t all_must). set_solver.
+    eapply cowt_iff_wt_nil. eassumption. }
+  destruct must_p'; eauto.
+  edestruct (ex p') as ((p'' , t'') & HypTr). now eapply elem_of_singleton.
+  inversion HypTr as [? ? ? ? tau_left | ? ? ? ? tau_right | ? ? ? ? ? ? ? act_left act_right]; subst.
+  - eapply lts_refuses_spec2 in stp'; eauto.
+  - destruct (lts_refuses_decidable t τ) as [refuses_t | not_refuses_t].
+    + eapply lts_refuses_spec2 in refuses_t. eauto. eauto with mdb.
+    + eapply (lts_refuses_spec2 (q ▷ t)); eauto.
+      exists (q , t''). eapply ParRight; eauto.
+  - eapply communication_enabled_co in act_left as (ν1 & ν2 & q' & t''' & duo & tr1 & tr2); eauto.
+    eapply (lts_refuses_spec2 (q ▷ t)); eauto. exists (q', t''').
+    eapply (ParSync ν1); eauto.
+Qed.
+
+Lemma stability_nbhvleqtwo_co
+  (X : gset P) (Y : gset Q) t :
+  ¬ outcome t
+    -> X must_pass_x t
+      -> X ₂≼꜀ₒ₋ₛₑₜ_ₐₛ Y
+        -> forall (q : Q), q ∈ Y -> ∃ q', (q, t) ⟶{τ} q'.
+Proof.
+  intros nhg hmx hleq q mem.
+  destruct (lts_refuses_decidable (q, t) τ).
+  - exfalso. apply (unoutcome_must_st_nleqx_co X Y t nhg hmx); eauto.
+  - eapply lts_refuses_spec1 in n as (t' & hl). eauto.
+Qed.
+
+Lemma unoutcome_acnv_mu_co (X : gset P) (t t' : T) :
+  X must_pass_x t
+    -> forall μ p, p ∈ X
+      -> t ⟶[μ] t'
+          -> ¬ outcome t -> ¬ outcome t' -> p ⇓ᶜᵒ [μ].
+Proof.
+  intros hmx μ p mem l not_happy not_happy'.
+  dependent induction hmx.
+  - contradiction.
+  - edestruct (mustx_terminate_unoutcome X t) as [happy | finish]; eauto with mdb.
+    contradiction.
+    eapply cocnv_act. eauto.
+    intros q w.
+    assert (h1 : cowt_set_from_pset_spec1 X μ {[q]}).
+    exists p. split; set_solver.
+    assert (h2 : {[q]} ≠ (∅ : gset P)) by set_solver.
+    set (hm := com t' μ {[ q ]} l h1 h2).
+    destruct (mustx_terminate_unoutcome _ _ hm).
+    + contradiction.
+    + eapply cocnv_nil. eapply H2. set_solver.
+Qed.
+
+(** ** Soundness for sets *)
+
+Lemma soundnessx_co
+  (X : gset P) (Y : gset Q) :
+  X ≼꜀ₒ₋ₛₑₜ_ₐₛ Y  -> X ⊑ₛₑₜ_ₘᵤₛₜᵢ Y.
+Proof.
+  intros (halt1 & halt2) t hmx. revert Y halt1 halt2.
+  dependent induction hmx; intros Y halt1 halt2.
+  - eauto with mdb.
+  - assert (HX0 : forall p, p ∈ X -> p ⇓ᶜᵒ []).
+    { intros p mem. eapply cocnv_nil.
+      destruct (mustx_terminate_unoutcome X t ltac:(eauto with mdb)) as [c|h]; [contradiction|].
+      eauto. }
+    assert (HYterm : forall q, q ∈ Y -> q ⤓).
+    { intros q mem. eapply equiv_cotermination. eapply halt1; eauto. }
+    assert (Y_conv : Y ⤓).
+    { eapply co_termination_set_for_all. exact HYterm. }
+    assert (Hbuild : forall Y0,
+      Y0 ⤓ ->
+      X ₁≼꜀ₒ₋ₛₑₜ_ₐₛ Y0 -> X ₂≼꜀ₒ₋ₛₑₜ_ₐₛ Y0 -> mustx Y0 t).
+    { intros Y0 conv0. induction conv0 as [Y0 tY0 IHY0]. intros hb1 hb2.
+      eapply mx_step.
+      - eauto.
+      - eapply stability_nbhvleqtwo_co; eauto with mdb.
+      - intros Y0' hspec1 hne.
+        set (Y0full := cowt_tau_set_from_pset Y0).
+        destruct (cowt_tau_set_from_pset_ispec Y0) as (Y0full_spec1 & Y0full_spec2).
+        destruct (decide (Y0full = ∅)) as [Hemp | Hnemp].
+        + exfalso. assert (Y0' ⊆ Y0full) as Hsub0.
+          { intros q memq. destruct (hspec1 q memq) as (p & memp & lstep).
+            eapply Y0full_spec2; eauto. }
+          set_solver.
+        + assert (hstep0 : Y0 ⟶ Y0full) by (split; [reflexivity | exact Hnemp]).
+          specialize (IHY0 Y0full hstep0).
+          destruct (bhvx_preserved_by_reduction_co X Y0 Y0full Y0full_spec1 (conj hb1 hb2))
+            as (hb1full & hb2full).
+          specialize (IHY0 hb1full hb2full).
+          assert (Y0' ⊆ Y0full) as Hsub0.
+          { intros q memq. destruct (hspec1 q memq) as (p & memp & lstep).
+            eapply Y0full_spec2; eauto. }
+          eapply mx_sub; eauto.
+      - intros t' l. eapply H0; eauto with mdb.
+      - intros t' μ Y0' ltr lcowtspec hne.
+        destruct (decide (outcome t')) as [ot'|not_ot'].
+        + eapply mx_now; assumption.
+        + assert (HA : forall p, p ∈ X -> p ⇓ᶜᵒ [μ]).
+          { intros; eapply unoutcome_acnv_mu_co; eauto with mdb. }
+          destruct (cowt_s_set_from_pset_ispec X μ HA) as (Xfull_spec1 & Xfull_spec2).
+          set (Xfull := cowt_s_set_from_pset X μ HA) in *.
+          assert (htX : forall p, p ∈ X -> terminate p).
+          { destruct (mustx_terminate_unoutcome X t ltac:(eauto with mdb)) as [c|h]; [contradiction|exact h]. }
+          edestruct (reverse_trace_inclusion_co X Y0 Y0' μ (conj hb1 hb2) HA lcowtspec hne)
+            as (X'' & X''spec1 & X''ne).
+          assert (X'' ⊆ Xfull) as Hsub.
+          { intros q memq. destruct (X''spec1 q memq) as (p & memp & wpq).
+            eapply Xfull_spec2; eauto. }
+          assert (Xfull_ne : Xfull ≠ ∅) by set_solver.
+          destruct (bhvx_preserved_by_external_action_co X Xfull μ Y0 Y0' htX lcowtspec
+            (conj Xfull_spec1 Xfull_spec2) (conj hb1 hb2)) as (hb1' & hb2').
+          eapply (H1 t' μ Xfull ltr Xfull_spec1 Xfull_ne); eauto. }
+    eapply Hbuild; eauto with mdb.
+Qed.
+
+End SoundnessAS_co.
+
+Section SoundnessCoNbEnabled.
+
+Context `{gLtsP : @gLtsEq P A H, !coFiniteImagegLts P A}.
+Context `{gLtsQ : !gLtsEq Q H, !gLtsCNenabled Q A, !coFiniteImagegLts Q A}.
+Context `{gLtsT : !gLtsEq T H, !Testing_Predicate outcome _}.
+
+Context `{AbsPT : @AbsAction P T FinA PreAct A H Φ 𝝳 _ _ }.
+Context `{AbsQT : @AbsAction Q T FinA PreAct A H Φ 𝝳 _ _ }.
+
+Context `{!Prop_of_Inter P T A dual}.
+Context `{!Prop_of_Inter Q T A dual}.
+
+Lemma soundness_co_nb_enabled_co
+  (p : P) (q : Q) : p ≼꜀ₒ₋ₐₛ q -> p ⊑ₘᵤₛₜᵢ q.
+Proof.
+  intros halt e hm.
+  eapply must_set_iff_must.
+  eapply (soundnessx_co ({[p]} : gset P)).
+  now eapply alt_set_singleton_iff_co.
+  now eapply must_set_iff_must.
+Qed.
+
+End SoundnessCoNbEnabled.
+
+(* Depends on [soundness_co_nb_enabled_co] (now proven above) — the
+   [gLtsCNenabled Q A] instance it needs is derived after the fact, via
+   [Unshelve], from [gLtsObaFW Q A]'s [boomerang] property. *)
+Lemma soundness_fw_co `{
+  gLtsEqP : @gLtsEq P A H, !coFiniteImagegLts P A,
+  gLtsEqQ : @gLtsEq Q A H, !coFiniteImagegLts Q A, gLtsObaQ : !gLtsOba Q, !gLtsObaFW Q A,
+  gLtsT : !gLtsEq T H, !Testing_Predicate outcome _}
+
+  `{AbsPT : @AbsAction P T FinA PreAct A H Φ 𝝳 _ _ }
+  `{AbsQT : @AbsAction Q T FinA PreAct A H Φ 𝝳 _ _ }
+
+  `{!Prop_of_Inter P T A dual}
+  `{!Prop_of_Inter Q T A dual}
+
+  (p : P) (q : Q) : p ≼꜀ₒ₋ₐₛ q -> p ⊑ₘᵤₛₜᵢ q.
+Proof.
+  eapply soundness_co_nb_enabled_co.
+  Unshelve.
+  eapply MkgLtsCNenabled. intros.
+  destruct (boomerang p1 η β) as (t & l1 & l2) ; eauto. symmetry;eauto.
+Qed.
+
+(** ** Soundness for LTSs that can be lifted to forwarders, co variant *)
+(* Depends on [soundness_fw_co] (below), which depends on
+   [soundness_co_nb_enabled_co]/[soundnessx_co] (set-LTS-based). *)
+(*
+Lemma soundness_co
+  `{@gLtsObaFB P A H gLtsEqP gLtsObaP, !FiniteOutputChain_LtsOba P, !FiniteImagegLts P A}
+  `{@gLtsObaFB Q A H gLtsEqQ gLtsObaQ, !FiniteOutputChain_LtsOba Q, !FiniteImagegLts Q A}
+  `{@gLtsObaFB T A H gLtsEqT gLtsObaT, !FiniteOutputChain_LtsOba T, !FiniteImagegLts T A}
+
+  `{ !Testing_Predicate outcome _}
+
+  {_ : Prop_of_Inter P T A dual}
+  {_ : Prop_of_Inter Q T A dual}
+
+  {_ : @Prop_of_Inter P (MO A) A fw_inter H _ MbgLts}
+  {_ : @Prop_of_Inter (P * MO A) T A dual H (inter_lts fw_inter) _}
+
+  {_ : @Prop_of_Inter Q (MO A) A fw_inter H _ MbgLts}
+  {_ : @Prop_of_Inter (Q * MO A) T A dual H (inter_lts fw_inter) _}
+
+  (* [soundness_fw_co], applied below at the forwarder-pair types [P * MO
+     A]/[Q * MO A], now needs [coFiniteImagegLts] at that level. Unlike
+     [FiniteImagegLts (P * MO A) A] (auto-derived from [FiniteImagegLts P
+     A] by [ForwarderConstruction.v]'s [gLtsMBFinite] instance), no such
+     forwarder-pair instance exists yet for [coFiniteImagegLts] (same gap
+     noted in [EquivalenceASco.v]/[CompletenessASco.v]), so it is assumed
+     directly here. *)
+  `{!coFiniteImagegLts (P * MO A) A}
+  `{!coFiniteImagegLts (Q * MO A) A}
+
+  `{AbsPT : @AbsAction P T FinA PreAct A H Φ 𝝳 _ _ }
+  `{AbsQT : @AbsAction Q T FinA PreAct A H Φ 𝝳 _ _ }
+
+  (p : P) (q : Q) : p ▷ ∅ ≼꜀ₒ₋ₐₛ q ▷ ∅ -> p ⊑ₘᵤₛₜᵢ q.
+Proof.
+  intros halt t hm.
+  eapply Lift.must_iff_must_fw in hm.
+  eapply Lift.must_iff_must_fw.
+  now eapply (soundness_fw_co (p ▷ ∅) (q ▷ ∅)).
+Qed.
+*)
